elect composition defined and verivied

theories/Compositional_Structures/Basic_Modules/Component_Types/Electoral_Module_Ref.thy
@@ -25,10 +25,10 @@ abbreviation elec_mod_rel_ref :: "('a \<times> 'a) set \<Rightarrow>
 
 abbreviation elec_mod_data_rel :: "('a \<times> 'a) set \<Rightarrow> 
 ('a Electoral_Module_Ref \<times> ('a set \<Rightarrow> 'a Profile \<Rightarrow> 'a Result nres)) set" where
-  "elec_mod_data_rel R \<equiv> \<langle>R\<rangle>finite_set_rel \<rightarrow> profile_rel 
+  "elec_mod_data_rel R \<equiv> \<langle>R\<rangle>set_rel \<rightarrow> profile_rel 
   \<rightarrow> \<langle>\<langle>R\<rangle>set_rel \<times>\<^sub>r \<langle>R\<rangle>set_rel \<times>\<^sub>r \<langle>R\<rangle>set_rel\<rangle>nres_rel"
 
-definition em_prof_nres ::
+(*definition em_prof_nres ::
   "('a \<times> 'a) set \<Rightarrow> ('a Electoral_Module_Ref \<times> ('a set \<Rightarrow> 'a Profile \<Rightarrow> 'a Result)) set"
   where em_prof_nres_internal_def: "em_prof_nres R \<equiv> 
   {(emref, em). \<forall> (A', A) \<in> \<langle>R\<rangle>finite_set_rel.
@@ -39,43 +39,31 @@ lemma em_prof_nres_def[refine_rel_defs]:
   "\<langle>R\<rangle>em_prof_nres \<equiv>  {(emref, em). \<forall> (A', A) \<in> \<langle>R\<rangle>finite_set_rel.
   \<forall> (pl, pr) \<in> profile_on_A_rel (A').
    (emref A' pl ,RETURN(em A pr)) \<in> \<langle>\<langle>R\<rangle>set_rel \<times>\<^sub>r \<langle>R\<rangle>set_rel \<times>\<^sub>r \<langle>R\<rangle>set_rel\<rangle>nres_rel}"
-  by (simp add: em_prof_nres_internal_def relAPP_def)
+  by (simp add: em_prof_nres_internal_def relAPP_def)*)
 
 
-
-definition aux_set_copy :: "'a set \<Rightarrow> 'a set nres" where
-  "aux_set_copy A \<equiv>  FOREACH A
-     (\<lambda> x cp. RETURN (insert x cp)) {}"
-
-lemma aux_set_copy_correct:
-  fixes A :: "'a set"
-  assumes fina: "finite A"
-  shows "aux_set_copy A \<le> SPEC(\<lambda> set. set = A)"
-  unfolding aux_set_copy_def
-  apply (refine_vcg FOREACH_rule[where I = "\<lambda>it s. s = A - it"])
-  by (auto simp add: fina)
 
 
 
 definition elect_monadic ::
   "'a Electoral_Module_Ref \<Rightarrow> 'a set \<Rightarrow> 'a Profile_List \<Rightarrow> 'a set nres" where
   "elect_monadic m A p \<equiv> do {
-    result <- m A p;
-    RETURN (elect_r result)
+    (mel, mrej, mdef) <- m A p;
+    RETURN (mel)
   }"
 
 definition defer_monadic ::
   "'a Electoral_Module_Ref \<Rightarrow> 'a set \<Rightarrow> 'a  Profile_List \<Rightarrow> 'a set nres" where
   "defer_monadic m A p \<equiv> do {
-    result <- m A p;
-    RETURN (defer_r result)
+    (mel, mrej, mdef) <- m A p;
+    RETURN (mrej)
   }"
 
 definition reject_monadic ::
   "'a Electoral_Module_Ref \<Rightarrow> 'a set \<Rightarrow> 'a  Profile_List \<Rightarrow> 'a set nres" where
   "reject_monadic m A p \<equiv> do {
-    result <- m A p;
-    RETURN (reject_r result)
+    (mel, mrej, mdef) <- m A p;
+    RETURN (mdef)
   }"
 
 
@@ -87,9 +75,11 @@ lemma elect_monadic_correct_aux:
   shows "elect_monadic emref A pl \<le> SPEC (\<lambda> es. es = (elect em A pr))"
   unfolding elect_monadic_def
   apply refine_vcg
-  unfolding SPEC_eq_is_RETURN(2)[symmetric]
-  using emrefc
-  by (simp add: SPEC_trans) 
+  using emrefc unfolding
+RETURN_SPEC_conv[symmetric]  using  SPEC_trans  case_prod_beta'
+  by (metis (mono_tags) RETURN_rule order_class.order_eq_iff)
+
+  
 
 lemma elect_monadic_correct:
   fixes emref :: "'a Electoral_Module_Ref"
@@ -112,59 +102,14 @@ proof (intro frefI, clarsimp, refine_vcg, rename_tac A pl pr)
   assume profa: "profile A pr"
   have " emref A pl \<le> RETURN (em A pr)"
     using fina prel profa emrefc[THEN frefD, THEN nres_relD] by auto
-  thus "emref A pl \<le> SPEC (\<lambda>result. RETURN (elect_r result) \<le> SPEC (\<lambda>c. (c, elect em A pr) \<in> Id))"
-    by (simp add: SPEC_trans)
+  thus "emref A pl
+       \<le> SPEC (\<lambda>x. (case x of (mel, mrej, mdef) \<Rightarrow> RETURN mel) \<le> SPEC (\<lambda>c. (c, elect em A pr) \<in> Id))"
+     using emrefc unfolding
+       RETURN_SPEC_conv[symmetric]  using  SPEC_trans  case_prod_beta' IdI RETURN_rule
+     by (metis (no_types, lifting) )
+ 
  qed
     
-lemma defer_monadic_correct:
-  fixes emref :: "'a Electoral_Module_Ref"
-  and em :: "'a Electoral_Module"
-  assumes emrefc: "(uncurry emref, uncurry (RETURN oo em)) \<in> 
-  ([\<lambda> (A, pl). finite_profile A
-            pl]\<^sub>f (\<langle>Id\<rangle>set_rel \<times>\<^sub>r profile_rel)
-   \<rightarrow> \<langle>\<langle>Id\<rangle>set_rel \<times>\<^sub>r \<langle>Id\<rangle>set_rel \<times>\<^sub>r \<langle>Id\<rangle>set_rel\<rangle>nres_rel)"
-  shows "(uncurry (defer_monadic emref), uncurry (RETURN oo (defer em))) \<in>
-    ([\<lambda> (A, pl). finite_profile A
-            pl]\<^sub>f (\<langle>Id\<rangle>set_rel \<times>\<^sub>r profile_rel)
-   \<rightarrow> \<langle>\<langle>Id\<rangle>set_rel\<rangle>nres_rel)"
-  unfolding defer_monadic_def comp_apply
-proof (intro frefI, clarsimp, refine_vcg, rename_tac A pl pr)
-  fix A :: "'a set"
-  fix pl :: "'a Profile_List"
-  fix pr :: "'a Profile"
-  assume prel: "(pl, pr) \<in> profile_rel"
-  assume fina: "finite A"
-  assume profa: "profile A pr"
-  have " emref A pl \<le> RETURN (em A pr)"
-    using fina prel profa emrefc[THEN frefD, THEN nres_relD] by auto
-  thus "emref A pl \<le> SPEC (\<lambda>result. RETURN (defer_r result) \<le> SPEC (\<lambda>c. (c, defer em A pr) \<in> Id))"
-    by (simp add: SPEC_trans)
-qed
-
-lemma reject_monadic_correct:
-  fixes emref :: "'a Electoral_Module_Ref"
-  and em :: "'a Electoral_Module"
-  assumes emrefc: "(uncurry emref, uncurry (RETURN oo em)) \<in> 
-  ([\<lambda> (A, pl). finite_profile A
-            pl]\<^sub>f (\<langle>Id\<rangle>set_rel \<times>\<^sub>r profile_rel)
-   \<rightarrow> \<langle>\<langle>Id\<rangle>set_rel \<times>\<^sub>r \<langle>Id\<rangle>set_rel \<times>\<^sub>r \<langle>Id\<rangle>set_rel\<rangle>nres_rel)"
-  shows "(uncurry (reject_monadic emref), uncurry (RETURN oo (reject em))) \<in>
-    ([\<lambda> (A, pl). finite_profile A
-            pl]\<^sub>f (\<langle>Id\<rangle>set_rel \<times>\<^sub>r profile_rel)
-   \<rightarrow> \<langle>\<langle>Id\<rangle>set_rel\<rangle>nres_rel)"
-  unfolding reject_monadic_def comp_apply
-proof (intro frefI, clarsimp, refine_vcg, rename_tac A pl pr)
-  fix A :: "'a set"
-  fix pl :: "'a Profile_List"
-  fix pr :: "'a Profile"
-  assume prel: "(pl, pr) \<in> profile_rel"
-  assume fina: "finite A"
-  assume profa: "profile A pr"
-  have " emref A pl \<le> RETURN (em A pr)"
-    using fina prel profa emrefc[THEN frefD, THEN nres_relD] by auto
-  thus "emref A pl \<le> SPEC (\<lambda>result. RETURN (reject_r result) \<le> SPEC (\<lambda>c. (c, reject em A pr) \<in> Id))"
-    by (simp add: SPEC_trans)
-qed    
     
 
 locale set_select_imp = 
