theories/Compositional_Structures/Basic_Modules/Elect_Module_Ref.thy
@@ -7,6 +7,20 @@ begin
  \<comment> \<open>The elect module should not return just the reference to all alternatives
   but a deep copy\<close>
 
+definition aux_set_copy :: "'a set \<Rightarrow> 'a set nres" where
+  "aux_set_copy A \<equiv>  FOREACH A
+     (\<lambda> x cp. RETURN (insert x cp)) {}"
+
+lemma aux_set_copy_correct:
+  fixes A :: "'a set"
+  assumes fina: "finite A"
+  shows "aux_set_copy A \<le> SPEC(\<lambda> set. set = A)"
+  unfolding aux_set_copy_def
+  apply (refine_vcg FOREACH_rule[where I = "\<lambda>it s. s = A - it"])
+  by (auto simp add: fina)
+
+
+
 fun elect_module_ref :: "'a Electoral_Module_Ref" where
   "elect_module_ref A p = do {
    B <- aux_set_copy A;
@@ -14,29 +28,21 @@ fun elect_module_ref :: "'a Electoral_Module_Ref" where
 }"
 
 lemma elect_module_ref_correct:
-  shows "(elect_module_ref, (\<lambda> A p. SPEC (\<lambda> res. res = elect_module A p)))
-      \<in> elec_mod_relb Id"
+  shows "(uncurry elect_module_ref, uncurry (RETURN oo elect_module))
+      \<in> [\<lambda> (A, _). finite A]\<^sub>f (\<langle>Id\<rangle>set_rel \<times>\<^sub>r profile_rel)
+  \<rightarrow> \<langle>\<langle>Id\<rangle>set_rel \<times>\<^sub>r \<langle>Id\<rangle>set_rel \<times>\<^sub>r \<langle>Id\<rangle>set_rel\<rangle>nres_rel"
   unfolding elect_module_ref.simps elect_module.simps aux_set_copy_def
-  apply (intro fun_relI)
-proof (rename_tac A' A pl pr)
-  fix A' A:: "'a set"
+  apply (intro frefI fun_relI nres_relI) unfolding comp_apply
+  apply clarsimp
+proof (rename_tac A pl pr)
+  fix A:: "'a set"
   fix pl pr 
-  assume arel: "(A', A) \<in> \<langle>Id\<rangle>alt_set_rel"
-  from arel have aeq: "A' = A" by (auto simp add: alt_set_rel_def in_br_conv)
-  from arel have fina: "finite A" by (auto simp add: alt_set_rel_def in_br_conv)
-  from fina have refid: "(FOREACH A' (\<lambda>x cp. RETURN (insert x cp)) {} \<bind> (\<lambda>B. RETURN (B, {}, {})),
-        SPEC (\<lambda>res. res = (A, {}, {})))
-       \<in> \<langle>Id\<rangle>nres_rel"
+ assume fina: "finite A"
+  from fina show "FOREACH A (\<lambda>x cp. RETURN (insert x cp)) {} \<bind> (\<lambda>B. RETURN (B, {}, {})) \<le> RETURN (A, {}, {})"
     apply (refine_vcg)
-    apply (simp add: aeq)
+    apply (auto)
     using aux_set_copy_correct aux_set_copy_def
     by (metis singleton_conv)
-    show "(FOREACH A' (\<lambda>x cp. RETURN (insert x cp)) {} \<bind> (\<lambda>B. RETURN (B, {}, {})),
-        SPEC (\<lambda>res. res = (A, {}, {})))
-       \<in> \<langle>\<langle>Id\<rangle>set_rel \<times>\<^sub>r \<langle>Id\<rangle>set_rel \<times>\<^sub>r \<langle>Id\<rangle>set_rel\<rangle>nres_rel"
-      apply (refine_vcg)
-    using refid[THEN nres_relD] prod_rel_id set_rel_id
-    by simp
 qed
 
   
