theories/Compositional_Structures/Sequential_Composition_Ref.thy
@@ -4,64 +4,38 @@ theory Sequential_Composition_Ref
         Refine_Imperative_HOL.Sepref
 begin
 
-
-
-definition sequential_composition_ref :: "'a Electoral_Module_Ref \<Rightarrow> 'a Electoral_Module_Ref \<Rightarrow>
-        'a Electoral_Module_Ref" where
-"sequential_composition_ref m n A p = do {
-      new_A <- (defer_monadic m) A p;
-      new_p <- limit_profile_l new_A p;  
-                        
-      electmA  <- (elect_monadic m) A p;
-      electnA' <- (elect_monadic n) new_A new_p;
-      
-      rejectmA  <- (reject_monadic m) A p;
-      rejectnA' <- (reject_monadic n) new_A new_p;
-
-      defernA'  <- (defer_monadic n) new_A new_p;
-
-      RETURN (electmA \<union> electnA',rejectmA \<union> rejectnA',defernA')
-}"
-
-
 definition sequential_composition_ref_test :: "'a Electoral_Module_Ref \<Rightarrow> 'a Electoral_Module_Ref \<Rightarrow>
         'a Electoral_Module_Ref" where
 "sequential_composition_ref_test m n A p = do {
-      mresulte <- m A p;
-      mresultr <- m A p;
-      
-      m'result <- m A p;
-      
-      let newA = (defer_r (m'result));
+      (mel,mrej,mdef) <- m A p;
+ 
+      let newA = mdef;
       new_p <- limit_profile_l newA p;  
+    
+      (nel,nrej,ndef) <- n newA new_p;
       
-      nresulte <- n newA new_p;
-      nresultr <- n newA new_p;
-      nresultd <- n newA new_p;
-      
-      RETURN (elect_r mresulte \<union> elect_r nresulte, reject_r mresultr \<union> reject_r nresultr
-      , defer_r nresultd)
+      RETURN (mel \<union> nel, mrej \<union> nrej, ndef)
 }"
 
 locale seqcomp_impl =
   fixes m_ref :: "nat Electoral_Module_Ref"
-  fixes m_impl :: "(nat, unit) hashtable
+  fixes m_sep :: "(nat, unit) hashtable
       \<Rightarrow> (nat array \<times> nat) list
          \<Rightarrow> ((nat, unit) hashtable \<times> (nat, unit) hashtable \<times> (nat, unit) hashtable) Heap"
   fixes n_ref :: "nat Electoral_Module_Ref"
-  fixes n_impl :: "(nat, unit) hashtable
+  fixes n_sep :: "(nat, unit) hashtable
       \<Rightarrow> (nat array \<times> nat) list
          \<Rightarrow> ((nat, unit) hashtable \<times> (nat, unit) hashtable \<times> (nat, unit) hashtable) Heap"
   assumes 
-    m_impl: "(uncurry m_impl, uncurry m_ref)
+    m_impl: "(uncurry m_sep, uncurry m_ref)
         \<in> (alts_set_impl_assn)\<^sup>k *\<^sub>a profile_impl_assn\<^sup>k \<rightarrow>\<^sub>a result_impl_assn"  
     and
-    n_impl: "(uncurry n_impl, uncurry n_ref)
+    n_impl: "(uncurry n_sep, uncurry n_ref)
         \<in> (alts_set_impl_assn)\<^sup>k *\<^sub>a profile_impl_assn\<^sup>k \<rightarrow>\<^sub>a result_impl_assn"
 
 begin
 
-  lemma this_loc: "seqcomp_impl m_ref m_impl n_ref n_impl" by unfold_locales
+  lemma this_loc: "seqcomp_impl m_ref m_sep n_ref n_sep" by unfold_locales
 
 sepref_register "m_ref" :: "nat Electoral_Module_Ref"
 declare m_impl [sepref_fr_rules]
@@ -98,14 +72,13 @@ n_ref_correct: "(uncurry n_ref, uncurry (RETURN oo n)) \<in>
 begin
 
 lemma seq_comp_correct:
-  shows "(uncurry (sequential_composition_ref m_ref n_ref),
+  shows "(uncurry (sequential_composition_ref_test m_ref n_ref),
   uncurry (RETURN oo (sequential_composition m n)))
   \<in>   ([\<lambda> (A, pl). finite_profile A
             pl]\<^sub>f (\<langle>nat_rel\<rangle>set_rel \<times>\<^sub>r profile_rel)
    \<rightarrow> \<langle>\<langle>nat_rel\<rangle>set_rel \<times>\<^sub>r \<langle>nat_rel\<rangle>set_rel \<times>\<^sub>r \<langle>nat_rel\<rangle>set_rel\<rangle>nres_rel)"
-  unfolding sequential_composition_ref_def
-proof (intro frefI nres_relI,clarsimp simp del: limit_profile.simps, rename_tac A pl pr,
-    unfold SPEC_eq_is_RETURN(2)[symmetric], refine_vcg)
+  unfolding sequential_composition_ref_test_def
+proof (intro frefI nres_relI,clarsimp simp del: limit_profile.simps, rename_tac A pl pr)
   fix A :: "nat set"
   fix pl :: "nat Profile_List"
   fix pr :: "nat Profile"
@@ -113,11 +86,7 @@ proof (intro frefI nres_relI,clarsimp simp del: limit_profile.simps, rename_tac 
   assume fina: "finite A"
   assume profa: "profile A pr"
   note mrc = m_ref_correct[THEN frefD, THEN nres_relD]
-  note drc = defer_monadic_correct[THEN frefD, THEN nres_relD]
-  from fina prel profa have "defer_monadic m_ref A pl \<le> SPEC (\<lambda> dset. dset = defer m A pr)"
-    unfolding SPEC_eq_is_RETURN(2) using m_ref_correct drc[where emref2 = m_ref and em2 = m and x1 = "(A, pl)"
-        and y1 = "(A, pr)"]
-    by auto
+  note nrc = n_ref_correct[THEN frefD, THEN nres_relD]
   let ?new_A = "defer m A pr"
   let ?new_p = "limit_profile ?new_A pr"
   have fin_def: "finite ?new_A"
@@ -127,33 +96,55 @@ proof (intro frefI nres_relI,clarsimp simp del: limit_profile.simps, rename_tac 
     "profile (defer m A pr) (limit_profile (defer m A pr) pr)"
     using def_presv_fin_prof fina profa module_m
     by metis
-  from fina prel profa have "limit_profile_l ?new_A pl \<le> 
+  from fina prel profa have limitref: "limit_profile_l ?new_A pl \<le> 
     \<Down> profile_rel (SPEC (\<lambda> lim. lim = limit_profile (defer m A pr) pr))"
-    unfolding SPEC_eq_is_RETURN(2) using limitp_correct[THEN frefD, THEN nres_relD, where  x1 = 
-        "(A, pl)"
-        and y1 = "(A, pr)"]
-    unfolding comp_apply 
-  from prel fina profa show "defer_monadic m_ref A pl
-       \<le> SPEC (\<lambda>new_A.
-                   limit_profile_l new_A pl \<bind>
-                   (\<lambda>new_p.
-                       elect_monadic m_ref A pl \<bind>
-                       (\<lambda>electmA.
-                           elect_monadic n_ref new_A new_p \<bind>
-                           (\<lambda>electnA'.
-                               reject_monadic m_ref A pl \<bind>
-                               (\<lambda>rejectmA.
-                                   reject_monadic n_ref new_A new_p \<bind>
-                                   (\<lambda>rejectnA'.
-                                       defer_monadic n_ref new_A new_p \<bind>
-                                       (\<lambda>defernA'.
-                                           SPEC
-                                            (\<lambda>x. x = (electmA \<union> electnA', rejectmA \<union> rejectnA',
-  defernA'))))))))
-                   \<le> SPEC (\<lambda>x. x = (let new_A = defer m A pr; new_p = limit_profile new_A pr
-                                     in (elect m A pr \<union> elect n new_A new_p,
-                                         reject m A pr \<union> reject n new_A new_p, defer n new_A new_p))))"
- 
+    unfolding SPEC_eq_is_RETURN(2) using limitp_correct[THEN frefD, THEN nres_relD, where
+         y1 = "((defer m A pr), pr)" and x1 = "((defer m A pr), pl)"]
+    unfolding comp_apply
+    by (simp add: fin_def) 
+  have "sequential_composition m n A pr =
+      (let (mel,mrej,mdef) = m A pr in
+      
+      let newA = (mdef) in
+      let new_p = limit_profile newA pr in
+    
+      let (nel,nrej,ndef) = n newA new_p in
+      
+      (mel \<union> nel, mrej \<union> nrej, ndef))"
+    unfolding sequential_composition.simps apply auto
+    by (metis (no_types, lifting) case_prod_beta')
+    
+  from prel fina profa prof_def_lim fin_def  have  "  m_ref A pl \<bind>
+       (\<lambda>(mel, mrej, mdef).
+           limit_profile_l mdef pl \<bind>
+           (\<lambda>new_p. n_ref mdef new_p \<bind> (\<lambda>(nel, nrej, ndef). RETURN (mel \<union> nel, mrej \<union> nrej, ndef))))
+       \<le> RETURN
+           (let (mel,mrej,mdef) = m A pr in
+      
+      let newA = (mdef) in
+      let new_p = limit_profile newA pr in
+    
+      let (nel,nrej,ndef) = n newA new_p in
+      
+      (mel \<union> nel, mrej \<union> nrej, ndef))"
+    apply (refine_vcg prel fina profa prof_def_lim fin_def 
+        limitp_correct[THEN frefD, THEN nres_relD] mrc nrc)
+   using limitp_correct[THEN frefD, THEN nres_relD] mrc nrc
+    sorry
+  show "  m_ref A pl \<bind>
+       (\<lambda>(mel, mrej, mdef).
+           limit_profile_l mdef pl \<bind>
+           (\<lambda>new_p. n_ref mdef new_p \<bind> (\<lambda>(nel, nrej, ndef). RETURN (mel \<union> nel, mrej \<union> nrej, ndef))))
+       \<le> RETURN
+           (let new_A = defer m A pr; new_p = limit_profile new_A pr
+            in (elect m A pr \<union> elect n new_A new_p, reject m A pr \<union> reject n new_A new_p,
+                defer n new_A new_p))"
+    apply (refine_vcg prel fina profa prof_def_lim fin_def 
+        limitp_correct[THEN frefD, THEN nres_relD] mrc nrc)
+    sorry
+qed
+
+lemmas sequence_correct = sequential_composition_sep.refine[FCOMP seq_comp_correct]
 
 end
 
