theories/Compositional_Structures/Elect_Composition_Ref.thy
@@ -10,22 +10,51 @@ definition
 
 thm "elector_sep_def"
 
-lemma elector_sep_impl: "seqcomp_impl m_ref m_impl elect_module_ref elect_module_sep"
+locale elector_impl =  
+  fixes m_ref :: "nat Electoral_Module_Ref"
+  fixes m_sep :: "(nat, unit) hashtable
+      \<Rightarrow> (nat array \<times> nat) list
+         \<Rightarrow> ((nat, unit) hashtable \<times> (nat, unit) hashtable \<times> (nat, unit) hashtable) Heap"
+  assumes 
+    m_impl: "(uncurry m_sep, uncurry m_ref)
+        \<in> (alts_set_impl_assn)\<^sup>k *\<^sub>a profile_impl_assn\<^sup>k \<rightarrow>\<^sub>a result_impl_assn"
+begin
+
+interpretation electori:  seqcomp_impl m_ref m_sep elect_module_ref elect_module_sep
   apply unfold_locales
-proof -
-  show "(uncurry elect_module_sep, uncurry elect_module_ref)
-    \<in> (hs.assn nat_assn)\<^sup>k *\<^sub>a
-       profile_impl_assn\<^sup>k \<rightarrow>\<^sub>a hs.assn nat_assn \<times>\<^sub>a hs.assn nat_assn \<times>\<^sub>a hs.assn nat_assn"
-    using elect_module_sep.refine by simp
-next
+  using elect_module_sep.refine m_impl by auto
 
-  oops
+lemmas elector_sep_refine =  electori.seqt_imp_refine
+
+end
+
+locale elector_ref = elector_impl +
+  fixes m :: "nat Electoral_Module"
+assumes module_m: "electoral_module m"
+assumes m_ref_correct: "(uncurry m_ref, uncurry (RETURN oo m)) \<in> 
+  ([\<lambda> (A, pl). finite_profile A
+            pl]\<^sub>f (\<langle>nat_rel\<rangle>set_rel \<times>\<^sub>r profile_rel)
+   \<rightarrow> \<langle>\<langle>nat_rel\<rangle>set_rel \<times>\<^sub>r \<langle>nat_rel\<rangle>set_rel \<times>\<^sub>r \<langle>nat_rel\<rangle>set_rel\<rangle>nres_rel)" 
+begin
+
+lemmas m_t_ref = m_impl[FCOMP m_ref_correct]
 
 
 
-interpretation electori:  seqcomp_impl m_ref m_impl elect_module_ref elect_module_sep
+interpretation elector: sequence_refine m_ref m_sep elect_module_ref elect_module_sep m elect_module
+  apply unfold_locales
+  subgoal using m_impl .
+  subgoal  using elect_module_sep.refine .
+  subgoal using module_m.
+  subgoal by simp
+  subgoal using m_ref_correct.
+  subgoal apply (intro frefI nres_relI) 
+    using elect_module_ref_correct[THEN frefD, THEN nres_relD]
+    unfolding comp_apply by auto
+  done
 
-  oops
+
+lemmas elector_sep_refine =  elector.sequence_correct
 
 
 end
