theories/Compositional_Structures/Sepref_Bindings.thy
@@ -36,6 +36,8 @@ sepref_decl_op (no_def) defer_equal_imp: "(defer_equal_condition)" ::
 
 
 
+
+
 locale refine_assns =
  notes  
        ballot_assn_def[symmetric,fcomp_norm_unfold]
@@ -48,22 +50,34 @@ begin
 
 
 sepref_decl_impl borda_impl: borda_elim_sepref.refine[FCOMP borda_ref_correct] 
-  by simp
+  by simp                                       
 
 
 
 sepref_decl_impl defer_eqal_condition_impl: defer_equal_condition_sep.refine .
 
+
+
+
 end
 
 
-locale seq_binding = seqcomp_impl + refine_assns
+
+locale seq_binding = sequence_refine + refine_assns
 begin
 
-sepref_decl_op  seq_comb: "sequential_composition  ::
-  'a Electoral_Module \<Rightarrow> 'a Electoral_Module \<Rightarrow> 'a Electoral_Module" :: 
-  "\<langle>(elec_mod_rel_orig A), \<langle>(elec_mod_rel_orig A), (elec_mod_rel_orig_nres A)\<rangle>fun_rel\<rangle>fun_rel" 
-  sorry
+sepref_decl_op (no_def)  seqref: "sequential_composition m n  ::
+  nat Electoral_Module" :: 
+  "(elec_mod_rel_orig A)" 
+  where "A = Id"
+  apply standard
+  apply (rule nres_relI)
+  by (auto)
+
+
+
+sepref_decl_impl seq_impl: sequential_composition_sep.refine[FCOMP seq_comp_correct]
+
 
   
 
